added infrastructure for EndToEnd declarative specs

src/EndToEnd.v
@@ -1,47 +1,360 @@
-Require Import List seq ssreflect ssrbool ssrnat ZArith eqtype.
+Require Import Show.
+Require Import AbstractGen SetOfOutcomes Arbitrary Property.
+Require Import ssreflect ssrbool eqtype.
 
-Require Import AbstractGen Property SetOfOutcomes.
 
+Definition resultCorrect (r : Result) : bool := 
+  match r with
+    | MkResult (Some res) expected _ _ _ _ => 
+      res == expected
+    | _ => true
+  end.
+
+Definition failure qp :=
+  match qp with
+    | MkProp (MkRose res _) => ~~ (resultCorrect res)
+  end.
+
+(* Maps a Property to a Prop *)
 Definition semProperty (P : Pred QProp) : Prop :=
   forall qp, P qp -> failure qp = false.
 
+(* Maps a Testable to a Prop i.e. gives an equivalent proposition to the 
+   property under test *)
 Definition semTestable {A : Type} {_ : @Testable Pred A} (a : A) : Prop :=
   semProperty (property a).
 
-Lemma semForAll : forall {A prop : Type} {H : Testable prop}
-    show (gen : Pred A) (pf : A -> prop),
-  semProperty (@forAll Pred _ _ _ H show gen pf) <->
-  (forall a : A, gen a -> (semProperty (property (pf a)))).
-Proof.
-  move => A prop Htest show gen pf. split => H'.  
-  - move => a Hgen.
-    unfold bindP, semProperty, forAll in * . move=> qp. simpl in *.
-    set qp' :=  
-      match qp with
-        | {| unProp := t |} =>
-          {| unProp := fmapRose
-                         (fun r : Result =>
-                            addCallback r
-                                        (PostFinalFailure Counterexample
-                                                          (fun _  _  =>
-                                                             0))) t |} end.
-    move /(_ qp') : H' => H' H''. 
-    have: failure qp' = false.
-    { apply H'.  rewrite /bindP.  exists a. split => //.
-      exists qp. split => //. }
-    rewrite /qp'. destruct qp as [[[]]]. compute. auto.
-  - unfold semProperty in * => qp Hforall.
-    unfold forAllShrink in Hforall. 
-    rewrite /forAll /= /fmapP /returnP in Hforall.
-    move : Hforall => [a [Hgen [qp' [Hprop Hret]]]]. 
-    apply H' in Hprop => //. subst. 
-    destruct qp' as [[[]]]. compute. auto.
- Qed.
+(* Lemmas about idempotent combinators i.e. combinators that do not change
+   the testing outcome *)
 
-Lemma semForAllShrink : forall {A prop : Type} {H : Testable prop}
-    show (gen : Pred A) (pf : A -> prop) shrink,
-  semProperty (@forAllShrink Pred _ _ _ H show gen shrink pf) <->
-  (forall a : A, gen a -> (semProperty (property (pf a)))).
+Lemma mapTotalResult_idemp: 
+  forall {prop : Type} {H : Testable prop} (f : Result -> Result) (p : prop),
+    (forall res, resultCorrect res = resultCorrect (f res)) -> 
+    ((semTestable p) <-> (semProperty (@mapTotalResult Pred _ _ _ f p))).
+Proof.
+  move=> prop H f p Hyp. 
+  rewrite /semTestable  /mapTotalResult /mapRoseResult /mapProp /semProperty.
+  split.
+  - move => H1 qp [qp' [/H1 Hprop H2]]. 
+    rewrite /returnP in H2. subst. rewrite /failure. 
+    destruct qp' as [[]]. simpl in *. by rewrite -Hyp.
+  - move=> H1 qp Hprop. 
+    set qp' := 
+      match qp with
+        | {| unProp := t |} => {| unProp := fmapRose f t |}
+      end.         
+    have: failure qp' = false.
+    { apply H1. rewrite fmapGen_def. exists qp; split => //. }
+    destruct qp as [[]]. simpl in *. by rewrite -Hyp.
+Qed.
+
+
+Lemma semCallback_idemp:
+  forall {prop : Type} {H : Testable prop} (cb : Callback) (p : prop), 
+    semProperty (callback cb p) <-> semTestable p.
+Proof.
+  move => prop tp cb p. rewrite /callback. 
+  split; move => H. 
+  - apply mapTotalResult_idemp in H => //;
+    by move => [? ? ? ? ? ?].
+  - apply mapTotalResult_idemp => //;
+    by move => [? ? ? ? ? ?].
+Qed.
+                                                             
+Lemma semWhenFail_idemp:
+  forall {prop : Type} {H : Testable prop} (s : String.string) (p : prop), 
+    semProperty (whenFail s p) <-> semTestable p.
+Proof.
+  move => prop H s p. by rewrite /whenFail semCallback_idemp. 
+Qed.
+
+  
+Lemma semPrintTestCase_idemp:
+  forall {prop: Type} {tp : Testable prop} (s: String.string) (p: prop),
+    semProperty (printTestCase s p) <-> semTestable p.
+Proof.
+  move => prop tp s p. by rewrite /printTestCase semCallback_idemp.
+Qed.
+
+(* our current assumption is this one *)
+Lemma semShrinking_idemp:
+  forall {prop A : Type} {H : Testable prop}
+         (shrinker : A -> list A) (x0 : A) (pf : A -> prop),
+    semProperty (shrinking shrinker x0 pf) <-> 
+    semTestable (pf x0).
 Proof.
   admit.
+Qed. 
+
+Lemma semCover_idemp: 
+  forall {prop : Type} {H : Testable prop} (b: bool) (n: nat) 
+         (s: String.string) (p : prop), 
+    semProperty (cover b n s p) <-> semTestable p.
+Proof.
+  move=> prop H b n s p. split. 
+  - rewrite /cover. case: b => //.   
+    move => H1. apply mapTotalResult_idemp in H1 => //.
+      by move => [? ? ? ? ? ?]. 
+  - move => H1. rewrite /cover. case: b => //.
+    apply mapTotalResult_idemp => //.
+      by move => [? ? ? ? ? ?].
+Qed.
+      
+Lemma semClassify_idemp:
+   forall {prop : Type} {H : Testable prop} (b: bool) (s: String.string) 
+          (p : prop), 
+    semProperty (classify b s p) <-> semTestable p.
+Proof.
+  move=> prop H b s p. by rewrite /classify semCover_idemp. 
+Qed.
+
+Lemma semLabel_idemp:
+   forall {prop : Type} {H : Testable prop} (s: String.string) 
+          (p : prop), 
+    semProperty (label s p) <-> semTestable p.
+Proof.
+  move=> prop H s p. by rewrite /label semClassify_idemp. 
+Qed.
+    
+Lemma semCollect_idemp:
+   forall {prop : Type} {H : Testable prop} (s: String.string) 
+          (p : prop), 
+    semProperty (collect s p) <-> semTestable p.
+Proof.
+  move=> prop H s p. by rewrite /collect semLabel_idemp. 
+Qed.
+
+
+(* equivalences for other combinators *)
+
+Lemma semBindGen: 
+  forall {A} (gen : Pred A) (p : A -> @Property Pred),
+    semProperty (bindGen gen p) <-> forall g, gen g -> semProperty (p g).
+Proof. 
+  move=> A gen prop. rewrite /semProperty. split.
+  - move => H g Hgen qp Hprop. apply H. 
+    rewrite bindGen_def. exists g. split => //.
+  - move => H qp [a [Hgen Hprop]]. eauto.
+Qed.
+
+Lemma semReturnGen: 
+  forall (p : QProp),
+    semProperty (returnGen p) <-> semProperty (property p).
+Proof. 
+  move=> p. rewrite /semProperty. split;
+  move => H qp Hprop; auto.
+Qed.
+
+Lemma semForAll : 
+  forall {A prop : Type} {H : Testable prop} 
+         show (gen : Pred A) (pf : A -> prop),
+  semProperty (@forAll Pred _ _ _ H show gen pf) <->
+  (forall a : A, gen a -> (semTestable (pf a))).
+Proof.  
+  move => A prop Htest show gen pf. split => H'.
+  - rewrite /forAll in H'. move/semBindGen : H' => H' a /H' Hgen.
+    by apply semPrintTestCase_idemp in Hgen.  
+  - rewrite /forAll in H' *. apply semBindGen => g Hgen.
+    rewrite semPrintTestCase_idemp. by apply H'.
+Qed.
+
+Lemma semPredQProp:
+  forall (p : Pred QProp), semTestable p <-> (semProperty p).
+Proof.  
+  move=> p. 
+  rewrite /semTestable /property /testGenProp /property /testProp semBindGen. 
+  split.
+  - move => H pq /H Hgen. rewrite returnGen_def /semProperty in Hgen.
+    by apply Hgen.
+  - move => H pq Hgen. rewrite returnGen_def /semProperty.
+    move => qp Heq; subst. rewrite /semProperty in H. by auto.
+Qed.
+
+Lemma semForAllShrink: 
+  forall {A prop : Type} {H : Testable prop}
+         show (gen : Pred A) (pf : A -> prop) shrink,
+    semProperty (@forAllShrink Pred _ _ _ H show gen shrink pf) <->
+    (forall a : A, gen a -> (semTestable (pf a))).
+Proof.
+  move => A prop H show gen pf shrink. split.
+  - rewrite /forAllShrink semBindGen. 
+    move=> H' a /H' Hgen. setoid_rewrite semShrinking_idemp in Hgen.
+    setoid_rewrite semPredQProp in Hgen.
+    by apply semPrintTestCase_idemp in Hgen.
+  - move=> H'. rewrite /forAllShrink semBindGen. move => a g. 
+    rewrite semShrinking_idemp. apply semPredQProp. 
+    rewrite semPrintTestCase_idemp. by auto. 
+Qed.
+
+(* equivalent Props for Testables *)
+
+Lemma semBool: 
+  forall (b : bool), (b = true) <-> semTestable b.
+Proof.   
+  move => b. case: b.
+  - split => //. compute. 
+    by move => _ qp Heq; subst. 
+  - split => //. compute.
+    set qp := {| unProp := returnRose (updReason failed "Falsifiable") |}.
+    move/(_ qp) => H. symmetry. apply H. reflexivity.
+Qed.
+
+Lemma semResult: 
+  forall (res: Result), resultCorrect res = true <-> semTestable res.
+Proof.  
+  rewrite /semTestable /property /testResult /semProperty.
+  move => res. split.
+  + move=> H [[res' l]] [Heq1 Heq2]; subst. by rewrite /failure H.
+  + move=> /(_ ({| unProp := returnRose res |})) /= H. 
+    apply Bool.negb_false_iff. by apply H.
+Qed.
+
+Lemma semUnit: 
+  forall (t: unit), True <-> semTestable t.
+Proof.
+  move => t. split => // _. compute. 
+  by move => qp Heq; subst.
+Qed.
+
+Lemma semQProp:
+  forall (qp: QProp),
+    failure qp = false <-> semTestable qp.
+Proof.
+  move => qp. rewrite /semTestable /semProperty /property 
+                      /testProp returnGen_def. 
+  split.
+  - by move => H qp' Heq; subst.
+  - auto.
+Qed.
+
+Lemma semGen: 
+  forall (P : Type) {H : Testable P} (gen: Pred P), 
+    (forall p, gen p -> semTestable p) <-> (semTestable gen).  
+Proof.
+  move=> P H gen. split.
+  - move => H'. rewrite /semTestable /semProperty. move=> qp prop. 
+    rewrite /property /testGenProp in prop. move : prop => [p [/H' Hgen Hprop]].
+    rewrite /semTestable /semProperty in Hgen. by auto.
+  - move=> Hsem qp Hgen. rewrite /semTestable /semProperty in Hsem *.
+    move => qp' Hprop. apply Hsem. rewrite /property /testGenProp bindGen_def.
+    exists qp. split => //.
+Qed.
+   
+Lemma semFun: 
+  forall {A prop : Type} {H1 : Show A} {H2 : Arbitrary A} {H3 : Testable prop}
+         (f : A -> prop),
+    semTestable f <-> 
+    (forall (a : A), @arbitrary _ _ Pred _ a -> semTestable (f a)).
+Proof.
+  move=> A prop H1 H2 H3 f. 
+  rewrite /semTestable /property /testFun.
+  split.
+  - move => /semForAllShrink H' a' /H' Gen. by auto.
+  - move => H'. apply semForAllShrink => a' /H' Hgen. by auto.
+Qed.
+  
+(* I think this is the strongest property we can get for polymorphic functions *)
+Lemma semPolyFun: 
+  forall {prop : Type -> Type} {H : Testable (prop nat)} (f : forall T, prop T),
+    (semTestable (f nat)) <-> (semTestable f).
+Proof.
+  move => prop H f. rewrite /semTestable {2}/property /testPolyFun. 
+  by rewrite semPrintTestCase_idemp.
+Qed.
+
+Lemma semPolyFunSet: 
+  forall {prop : Set -> Type} {H : Testable (prop nat)} (f : forall T, prop T),
+    (semTestable (f nat)) <-> (semTestable f).
+Proof.
+  move => prop H f. rewrite /semTestable {2}/property /testPolyFun. 
+  by rewrite semPrintTestCase_idemp.
+Qed.
+
+(* A typeclass so we can automate the application of the previous theorems
+  and get a readable Prop *)
+
+Class Provable (A : Type) {H: Testable A} : Type :=
+ {
+    semProp : A -> Prop;
+    _ : forall a, semProp a <-> semTestable a 
+  }.
+
+Program Instance proveResult : Provable Result :=
+  {|
+    semProp := resultCorrect
+  |}.
+Next Obligation.
+  by apply semResult. 
+Qed.
+
+Program Instance proveUnit : Provable unit :=
+  {|
+    semProp := fun _ => True
+  |}.
+Next Obligation.
+  by apply semUnit.
+Qed.
+
+Program Instance proveQProp : Provable QProp :=
+  {|
+    semProp qp := failure qp = false
+  |}.
+Next Obligation.
+  by apply semQProp.
+Qed.
+
+Program Instance proveBool : Provable bool :=
+  {|
+    semProp b :=  b = true
+  |}.
+Next Obligation.
+  by apply semBool.
+Qed.
+
+Program Instance proveGenProp {prop : Type} `{Provable prop} : 
+  Provable (Pred prop) :=
+  {| 
+    semProp g := (forall p, g p -> semProp p)
+  |}.
+Next Obligation.
+  destruct H0 as [semP proof]. rewrite /semProp. split.
+  - move => H'. apply semGen=> p Hgen. apply proof. by auto.
+  - move => /semGen H' p Hgen. apply proof. by auto.
+Qed.
+
+Program Instance proveFun {A prop: Type} `{Arbitrary A} `{Show A}
+        `{Provable prop}: Provable (A -> prop) :=
+  {|
+    semProp p := 
+      (forall a, 
+         @arbitrary _ _ Pred _ a -> 
+         semProp (p a))
+  |}.
+Next Obligation. 
+  destruct H2 as [semP proof]. rewrite /semProp. split.
+  - move=> H'. apply semFun => a' /H' Hgen. 
+    by apply proof.
+  - move=> H' a' Hgen. apply proof. by apply semFun.
+Qed. 
+
+Program Instance provePolyFun {prop : Type -> Type} `{Provable (prop nat)} : 
+  Provable (forall T, prop T) :=
+  {
+    semProp f := semProp (f nat)
+  }.
+Next Obligation.
+  destruct H0 as [semP proof]. rewrite /semProp. split.
+  - move=> /proof H'. by apply semPolyFun.
+  - move=> /semPolyFun H'. by apply proof.
+Qed.
+
+Program Instance provePolyFunSet {prop : Set -> Type} `{Provable (prop nat)} : 
+  Provable (forall T, prop T) :=
+  {
+    semProp f := semProp (f nat)
+  }.
+Next Obligation.
+  destruct H0 as [semP proof]. rewrite /semProp. split.
+  - move=> /proof H'. by apply semPolyFunSet.
+  - move=> /semPolyFunSet H'. by apply proof.
 Qed.
